Tests/Completeness/LoopCorridor.lean
@@ -1,0 +1,33 @@
+/-
+Copyright (c) 2026 Bangyen Pham. All rights reserved.
+Released under Apache 2.0 license as described in the file LICENSE.
+Authors: Bangyen Pham
+-/
+import LeanFunge.Theory.Completeness.LoopCorridor
+
+/-!
+# Generated Loop Corridor Tests
+-/
+
+namespace LeanFunge.Tests
+
+open LeanFunge.Completeness
+
+example :
+    (run 36 (loopCorridorStart 3 0)).map (fun s => s.stack) = some [Int.ofNat (encode 2 1)] :=
+  loop_corridor_back
+
+example : run 137 (loopCorridorStart 3 0) = none :=
+  loop_corridor_halts
+
+example :
+    (run 136 (loopCorridorStart 3 0)).map (fun s => s.stack) = some [Int.ofNat (encode 0 3)] :=
+  loop_corridor_stack
+
+example :
+    (run 136 (loopCorridorStart 3 0)).map (fun s => s.stack)
+      = (CMInstr.run loopProgram 10 (CMInstr.startCM 3 0)).map
+          (fun s => [Int.ofNat (encode s.c1 s.c2)]) :=
+  loop_corridor_simulation
+
+end LeanFunge.Tests
